# FORMULARIO

 > $\boxed{\begin{align*} \varphi(s) &= \det(sI-A) &\longrightarrow \mu_{i} \\ m(s) &= \text{m.c.m. denominatori } (sI-A)^{-1} &\longrightarrow m_{i} \end{align*} \ \bigg\} \ 1 \leq m_{i} \leq \mu_i}$

>  $\boxed{\displaystyle (sI-A)^{-1}=\frac{1}{\varphi(s)}\ \text{Adj}(sI-A)}$

> $\boxed{\displaystyle e^{At}=\mathcal{L}^{-1}\{(sI-A)^{-1}\}}$

 > $\underline{A \in \mathbb{R}^{2\times2}}: \quad \displaystyle \boxed{\begin{bmatrix} a_{11} & a_{12} \\ a_{21} & a_{22} \end{bmatrix}^{-1}=\frac{1}{\det(A)} \cdot \begin{bmatrix} a_{22} & -a_{12} \\ -a_{21} & a_{11} \end{bmatrix}} \quad \boxed{\text{Adj}(A)=\text{Adj}\begin{bmatrix} a_{11} & a_{12} \\ a_{21} & a_{22} \end{bmatrix} = \begin{bmatrix} a_{22} & -a_{12} \\ -a_{21} & a_{11} \end{bmatrix}}$

 > $\boxed{G(s) = C(sI-A)^{-1}B+D}$

> $\displaystyle \underline{\text{Poli distinti}}: \quad \boxed{F(s)=\sum_{i=1}^{n} \frac{K_{i}}{(s-p_{i})}} \quad \boxed{K_{i}=\lim_{s \to p_{i}} (s-p_{i})\cdot F(s)} \ \Rightarrow \ \boxed{f(t) = \sum_{i=1}^{n} K_{i}e^{p_{i}t} \ 1(t)}$

> $\underline{\text{Andamento Modi per }e^{p_{i}t} \text{, con }p_{i}=\sigma_{i}+j \omega_{i}}: \quad \boxed{\begin{array}{c|c|c|c}  &\sigma_{i}<0 & \sigma_{i}=0 & \sigma_{i}>0 \\ \hline  \omega=0 &\stackrel{\Large\text{convergente}}{\text{non oscillante}} & \stackrel{\Large\text{limitato}}{\text{non oscillante}} & \stackrel{\Large\text{divergente}}{\text{non oscillante}} \\ \hline \omega_{i} \neq 0 & \stackrel{\Large\text{convergente}}{\text{ oscillante}} & \stackrel{\Large\text{limitato}}{\text{oscillante}} & \stackrel{\Large\text{divergente}}{\text{oscillante}} \end{array}}$

> $\underline{\text{Andamento Modi per }t^{\ell}e^{p_{i}t} \text{, con }p_{i}=\sigma_{i}+j \omega_{i}}: \quad \boxed{\begin{array}{c|c|c|c}  &\sigma_{i}<0 & \sigma_{i}=0 & \sigma_{i}>0 \\ \hline  \ell =0 &\text{convergente} & \text{limitato} & \text{divergente}\\ \hline \ell > 0 & \text{convergente}& \text{divergente}& \text{divergente}\end{array}}$

>>  $\underline{\text{Modi poli complessi: }}\quad  \boxed{(K_{i}e^{p_{i}t}+\overline K_{i}e^{\overline{p_{i}}t})\ 1(t)=2[ \alpha_{i}e^{\sigma_{i}t} \cos (\omega_{1}t)-\beta_{i}e^{\sigma_{i}t} \sin (\omega_{i}t)]1(t)} \quad , \quad K_{i}=\alpha_{i}+j \beta_{i}$

> $\displaystyle \text{Teorema Valore Finale (TVF):} \quad \boxed{\lim_{t \to \infty} f(t) = \lim_{s \to \infty} sF(s)}$

> $\displaystyle \text{Teorema Residui esteso: } \quad \boxed{F(s) = K_{0}+\sum_{i=1}^{k} \sum_{i=1}^{m_{i}} \frac{K_{i \ell}}{(s-p_{i})^{\ell}} \quad , \ K_{0}=b_{n} \quad}$

