
#### Evoluzioni complessive
$$
\begin{cases}
x(t) = x_{\ell}(t) + x_{f}(t)  \\
y(t) = y_{\ell}(t) + y_{f}(t)
\end{cases}
 \quad , \quad
\underbrace{\begin{align*}
x_{\ell}(t)&= A^{t}x_{0} & & x_{f}(t)=\sum_{\tau=0}^{t-1} A^{t-\tau-1}Bu(\tau)\\
y_{\ell}(t)&= CA^{t} x_{0} & & y_{f}(t)=\sum_{\tau=0}^{t-1} CA^{t-\tau-1}Bu(\tau)+Du(t)
\end{align*}}_{\text{TD}}
\quad
\underbrace{\begin{align*}
x_{\ell}(t)&= e^{At}x_{0} & & x_{f}(t)=\int_{0}^{t} e^{A(t-\tau)}  Bu(\tau)\,d\tau\\
y_{\ell}(t)&= Ce^{At}x_{0} & & x_{f}(t)=\int_{0}^{t} Ce^{A(t-\tau)}  Bu(\tau)\,d\tau\\
\end{align*}}_{\text{TC}}
$$

#### ESPONENZIALE DI MATRICE
$$
e^{At} = \sum_{k=0}^{\infty} \frac{(At)^{k}}{k!} = \sum_{k=0}^{\infty} \frac{A^{k} \ t^{k}}{k!} = \sum_{k=0}^{\infty} T \Lambda^{k}T^{-1} \ \frac{t^{k}}{k!}= T\big( \underbrace{\sum_{k=0}^{\infty} \Lambda^{k} \frac{t^{k}}{k!}}_{e^{\Lambda t}}  \big)= T e^{\Lambda t} T^{-1}
$$
#### TRASFORMATA DI LAPLACE
$$
F(s) = \mathcal{L} \{ f(t)\} = \int_{0}^{\infty} f(t) e^{-st} \,dt
$$

$$
\begin{array} {|c|c|}
\hline \textcolor{blue}{SEGNALE}  & \textcolor{blue}{f(t)} & \textcolor{blue}{F(s)}  \\ 
\hline \text{Impulso unitario} & \delta(t) & 1 \\
\hline \text{Gradino unitario} & 1(t) & 1/s \\
\hline \text{Rampa unitaria} & t \cdot 1(t) & 1/s^{2} \\
\hline \text{Rampa parab. unitaria} & (t^2/2) \cdot 1(t) & 1/s^{3} \\
\hline \text{Esponenziale} & e^{at}1(t) & 1/(s-a) \\
\hline \text{Sinusoide} & \sin(\omega_0 t)1(t) & \omega_0/(s^2+\omega_0^2) \\
\hline \text{Cosinusoide} & cos(\omega_0 t)1(t) & s/(s^2+\omega_0^2) \\
\hline \text{Esponenziale } \times \text{monomio} & (t^{\ell}/\ell!)e^{at}1(t) & 1/(s-a)^{\ell+1} \\ \hline
\end{array} 
 \quad \quad \quad
 \begin{array} {|c|c|}
\hline \textcolor{blue}{PROPRIETA'}  & \textcolor{blue}{TEMPO} & \textcolor{blue}{LAPLACE}  \\ 
\hline \text{Linearit√†} & \mathcal{L}\{\alpha_1f_1(t)+\alpha_2f_2(t)\} & \alpha_1F_{1}(s)+\alpha_2F_2(s)\\
\hline \text{Traslazione in frequenza} & \mathcal{L}\{e^{\lambda t}f(t)\} & F(s-\lambda)\\
\hline \text{Derivata in frequenza} & \mathcal{L}\left\{t \ f(t)\right\} & -\frac{d}{ds}F(s)\\
\hline \text{Derivata nel tempo} & \mathcal{L}\left\{\frac{d}{dt}f(t)\right\} & sF(s)-f(0)\\
\hline \text{Integrazione nel tempo} & \mathcal{L}\left\{\int_{0}^{t} f(\tau) \,d\tau \right\} & \frac{F(s)}{s}\\
\hline \text{Convoluzione} & \mathcal{L}\{(f*g)(t)\} & F(s)G(s) \\ \hline
\end{array} 
$$
