$\varphi(s) = \det(sI-A)$

$Adj\left(\begin{bmatrix} a & b \\ c & d \end{bmatrix}\right) = \begin{bmatrix} d & -b \\ -c & a \end{bmatrix}$

$\displaystyle \begin{bmatrix} a & b  \\ c & d \end{bmatrix}^{-1} = \frac{1}{\varphi(s)} \cdot Adj\left(\begin{bmatrix} a & b \\ c & d \end{bmatrix}\right)$

$\displaystyle e^{At} = \mathcal{L}^{-1}\{(sI-A)^{-1}\}$

---
#### fratti semplici
$\displaystyle \mathcal{L}^{-1}\left\{\frac{n}{a \cdot b}\right\} = \frac{k_{1}}{a}-\frac{k_{2}}{b} = \frac{k_{1}\cdot b+k_{2}\cdot a}{a\cdot b} \Rightarrow k_{1}\cdot b+k_{2}\cdot a=n \implies \begin{cases} \dots \\ \dots \end{cases} = \begin{cases} k_{1}=\dots \\ k_2 = \dots \end{cases}$
$\begin{align*} \mathcal{L}^{-1}\left\{\frac{1}{(s-a_{1})(s-a_{2}) \cdots(s-a_{n})}{}\right\} &= \frac{K_{1}}{(s-a_{1})}+\frac{K_{2}}{(s-a_{2})}+\dots-\frac{K_{n}}{(s-a_{n})} \\ &= K_{1} \mathcal{L}^{-1}\left\{\frac{1}{(s-a_{1})}\right\}+K_{2}\mathcal{L}^{-1}\left\{\frac{1}{(s-a_{2})}\right\}+ K_{n}\mathcal{L}^{-1}\left\{\frac{1}{(s-a_{n})}\right\} \end{align*}$
##### Teorema dei Residui e modi evoluzione
$\displaystyle \overbrace{F(s)}^{\stackrel{\large \text{str. propria+}}{\text{poli distinti}}} = \sum_{i=1}^{n} \frac{K_{i}}{s-p_{i}} = \sum_{i=1}^{n} \frac{\lim_{s \to p_{i}} (s-p_{i})\cdot F(s)}{s-p_{i}} \longleftrightarrow \mathcal{L}^{-1}\left\{\sum_{i=1}^{n} \frac{K_{i}}{s-p_{i}}\right\} = \sum_{i=1}^{n} \underbrace{K_{i}}_{\boxed{\text{residui}}}\cdot \overbrace{e^{p_{i}}}^{\boxed{\text{modi}}}1(t)=f(t)$

---
#### FUNZIONI RAZIONALI
$\displaystyle F(s) = \frac{b(s)}{a(s)} = \Rightarrow \begin{cases} \text{grado } b(s) < \text{grado } a(s) \to \text{strettamente propria}  \\ \text{grado } b(s) = \text{grado } a(s) \to \text{semplicemente propria} \end{cases}$
- $a(s)$ polinomio monico ($a_{n}=1$)  $\to$ sempre riconducibili a questo caso



